fix_on_join_cont' (for squnion instead of fmap_join)

Denotational-HeapExtend.thy
@@ -1,5 +1,5 @@
 theory "Denotational-HeapExtend"
-  imports "Denotational-Common"
+  imports "Denotational-Common" "HOLCF-Set" "HOLCF-Down-Closed"
 begin
 
 definition heapExtendJoin :: "Env \<Rightarrow> heap \<Rightarrow> (exp \<Rightarrow> Env \<Rightarrow> Value)  \<Rightarrow> (var, Value) fmap"
@@ -36,13 +36,285 @@ case False
   thus ?thesis unfolding heapExtendJoin_def apply (subst if_not_P, assumption)+ ..
 qed
 
+definition heapExtendJoin_cond
+  where "heapExtendJoin_cond h eval \<rho> = ((fdom \<rho> \<inter> fst ` set h) = {})"
 
+consts compatible_with_heap_and_env :: "heap \<Rightarrow> (exp \<Rightarrow> Env \<Rightarrow> Value) \<Rightarrow> Env \<Rightarrow> Env set"
 
 lemma heapExtendJoin_def3:
   "heapExtendJoin \<rho> h eval =
-    (if heapExtendMeed_cond h eval \<rho>
+    (if heapExtendJoin_cond h eval \<rho>
     then fix_on (compatible_with_heap_and_env h eval \<rho>) (\<lambda> \<rho>'. fmap_join \<rho> (heapToEnv h (\<lambda> e. eval e \<rho>')))
     else fempty)"
+sorry
+
+lemma subpcpo_compat_h_e:
+  "subpcpo (compatible_with_heap_and_env h ESem x)" sorry
+
+lemma closed_on_compat_h_e:
+  "closed_on (compatible_with_heap_and_env h ESem x)
+     (\<lambda>\<rho>'. fmap_join x (heapToEnv h (\<lambda>e. ESem e \<rho>')))" sorry
+
+lemma cont_on_compat_h_e:
+  "cont_on (compatible_with_heap_and_env h ESem x)
+     (\<lambda>\<rho>'. fmap_join x (heapToEnv h (\<lambda>e. ESem e \<rho>')))" sorry
+
+lemma compt_h_eD:
+  "\<rho> \<in> compatible_with_heap_and_env h ESem x \<Longrightarrow> compatible_fmap x (heapToEnv h (\<lambda>e. ESem e \<rho>))" sorry
+
+lemma bottom_of_compat_h_e:
+  "bottom_of (compatible_with_heap_and_env h ESem x) = fmap_bottom (fdom x \<union> fst ` set h)" sorry
+
+lemma heapExtendJoin_mono':
+  assumes "\<And> e. e \<in> snd ` set h \<Longrightarrow> cont (ESem e)"
+  shows "monofun (\<lambda>\<rho>. heapExtendJoin \<rho> h ESem)"
+proof (rule monofunI)
+case (goal1 x y)
+  hence [simp]:"fdom y = fdom x"
+    by (metis fmap_below_dom)
+  have subset:
+    "compatible_with_heap_and_env h ESem y \<subseteq> compatible_with_heap_and_env h ESem x" sorry
+  have same_bottom:
+    "bottom_of (compatible_with_heap_and_env h ESem x) = bottom_of (compatible_with_heap_and_env h ESem y)"
+    by (simp add: bottom_of_compat_h_e)
+
+  show ?case
+  proof(cases "fdom x \<inter> (fst ` set h) = {}")
+  case True[simp]
+    show ?thesis
+      unfolding heapExtendJoin_def3
+      unfolding heapExtendJoin_cond_def
+      apply (simp)
+      apply (rule parallel_fix_on_ind[OF subpcpo_compat_h_e subpcpo_compat_h_e _ closed_on_compat_h_e cont_on_compat_h_e  closed_on_compat_h_e cont_on_compat_h_e])
+      apply (rule adm_is_adm_on, simp)
+      apply (subst same_bottom, rule below_refl)
+      apply (drule compt_h_eD)+
+      apply (erule (1) fmap_join_mono[OF _ _ `x \<sqsubseteq> y` ])
+      apply (erule cont2monofunE[OF cont2cont_heapToEnv,rotated ])
+      apply (erule assms(1))
+      done
+  next
+  case False
+    thus ?thesis
+      unfolding heapExtendJoin_def3
+      unfolding heapExtendJoin_cond_def
+      by simp
+  qed
+qed
+
+(* More special version first, just to check proof *)
+lemma fix_join_cont':
+  fixes F :: "'a::pcpo \<Rightarrow> 'a"
+  assumes "chain Y"
+  assumes "cont F"
+  assumes "\<And> y::'a. cont (\<lambda>x. y \<squnion> x)"
+  assumes "\<And> y::'a. cont (\<lambda>x. x \<squnion> y)"
+  shows "(\<mu> x. (\<Squnion>i. Y i) \<squnion> F x) \<sqsubseteq> (\<Squnion> i. (\<mu> x. Y i \<squnion> F x))"
+  apply (rule Fix.fix_least_below)
+  apply (subst beta_cfun[OF cont_compose[OF assms(3) assms(2)]])
+  apply (subst cont2contlubE[OF assms(2)])
+  apply (rule ch2ch_cont[OF _ `chain Y`])
+  apply (rule cont_compose[OF cont_Rep_cfun2 cont2cont_LAM]) 
+  apply (rule cont_compose[OF assms(3) assms(2)])
+  apply (rule assms(4))
+  
+  apply (subst cont2contlubE[OF assms(3)])
+  defer
+  apply (subst cont2contlubE[OF assms(4) `chain Y`])
+  apply (subst diag_lub)
+  prefer 3
+  apply (subst Fix.fix_eq) back
+  apply (subst beta_cfun[OF cont_compose[OF assms(3) assms(2)]])
+  apply (rule below_refl)
+  apply (rule ch2ch_cont[OF _ `chain Y`])
+  apply (rule cont_compose[OF assms(3)])
+  apply (rule cont_compose[OF `cont F`])
+  apply (rule cont_compose[OF cont_Rep_cfun2 cont2cont_LAM]) 
+  apply (rule cont_compose[OF assms(3) assms(2)])
+  apply fact
+  apply (rule ch2ch_cont[OF _ `chain Y`])
+  apply fact
+  apply (rule ch2ch_cont[OF _ `chain Y`])
+  apply (rule cont_compose[OF `cont F`])
+  apply (rule cont_compose[OF cont_Rep_cfun2 cont2cont_LAM]) 
+  apply (rule cont_compose[OF assms(3) assms(2)])
+  apply fact
+  done
+
+lemma fix_on_join_cont':
+  fixes F :: "'a::pcpo \<Rightarrow> 'a"
+  assumes "subpcpo S'"
+  assumes pcpo_i: "\<And> i. subpcpo (S i)"
+  assumes "down_closed S'"
+  assumes ss': "\<And> i. S' \<subseteq> S i"
+  assumes same_bottoms[simp]: "\<And> i. bottom_of (S i) = bottom_of S'"
+  assumes "chain Y"
+  assumes "cont F"
+  assumes compat: "\<And> i x. x \<in> S i \<Longrightarrow> compatible (Y i) (F x)"
+  assumes cl: "\<And> i. closed_on (S i) (\<lambda>x. Y i \<squnion> F x)"
+  assumes cl': " closed_on S' (\<lambda>x. (\<Squnion> i. Y i) \<squnion> F x)"
+
+  shows "fix_on S' (\<lambda> x. (\<Squnion>i. Y i) \<squnion> F x) \<sqsubseteq> (\<Squnion> i. (fix_on (S i) (\<lambda> x. Y i \<squnion> F x)))" (is "_ \<sqsubseteq> Lub ?F")
+proof-
+  interpret subpcpo S' by fact
+  interpret down_closed S' by fact
+
+  note compat' = admD[OF compatible_adm1 `chain Y` compat[OF subsetD[OF ss']]]
+
+  have coF: "cont_on S' F" by (rule cont_is_cont_on[OF `cont F`])
+
+  have co: "\<And> i. cont_on (S i) (\<lambda>x. Y i \<squnion> F x)"
+  proof(rule subpcpo.cont_onI2[OF pcpo_i])
+  case goal1 show ?case
+    by (rule monofun_onI, erule (2) join_mono[OF compat compat below_refl cont2monofunE[OF `cont F`]])
+  next
+  case (goal2 i Y)
+    hence "chain Y" by (metis chain_on_is_chain)
+    show ?case
+      apply (rule subst[OF cont2contlubE[OF `cont F` `chain Y`, symmetric]])
+      apply (subst join_cont2[OF ch2ch_cont[OF `cont F` `chain Y`] compat[OF chain_on_is_on[OF goal2(1)]]])
+      apply (rule below_refl)
+    done
+  qed
+
+  have co': "cont_on S' (\<lambda>x. (\<Squnion> i. Y i) \<squnion> F x)"
+  proof(rule cont_onI2)
+  case goal1 show ?case
+    by (rule monofun_onI, rule join_mono[OF compat' compat' below_refl cont2monofunE[OF `cont F`]])
+  next
+  case (goal2 Y)
+    hence "chain Y" by (metis chain_on_is_chain)
+    show ?case
+      apply (rule subst[OF cont2contlubE[OF `cont F` `chain Y`, symmetric]])
+      apply (subst join_cont2[OF ch2ch_cont[OF `cont F` `chain Y`] compat'[OF chain_on_is_on[OF goal2(1)]]])
+      apply (rule below_refl)
+    done
+  qed
+
+  have co'': "\<And> i. cont_on S' (\<lambda>x. Y i \<squnion> F x)"
+    by (rule cont_on_subset[OF co ss'])
+  have cl'': "\<And> i. closed_on S' (\<lambda>x. Y i \<squnion> F x)"
+    by (rule closed_onI, rule down_closedE[OF
+        closed_onE[OF cl']
+        join_mono[OF
+          compat[OF subsetD[OF ss']]
+          compat'
+          is_ub_thelub[OF `chain Y`]
+          below_refl]])
+
+  have compat'': "\<And>j i. compatible (Y j) (F (?F i))"
+    apply (rule compat)
+    apply (rule subsetD[OF ss'])
+    apply (subst fix_on_same[OF pcpo_i subpcpo_axioms cl co cl'' co'' same_bottoms])
+    apply (rule fix_on_there[OF co'' cl''])
+    done
+
+  have  "fix_on S' (\<lambda>x. (Lub Y) \<squnion> F x) \<in> S'"
+    by (rule fix_on_there[OF co' cl'])
+  moreover
+  have "\<And> i. fix_on (S i) (\<lambda>x. Y i \<squnion> F x) \<sqsubseteq> fix_on S' (\<lambda>x. (Lub Y) \<squnion> F x)"
+    apply (rule fix_on_mono2[OF pcpo_i subpcpo_axioms cl co cl' co'])
+    apply simp
+    apply (erule (2) join_mono[OF
+        compat
+        compat'
+        is_ub_thelub[OF `chain Y`]
+        cont2monofunE[OF `cont F`]])
+    done
+  ultimately
+  have F_in_S': "\<And> i. fix_on (S i) (\<lambda>x. Y i \<squnion> F x) \<in> S'"
+    by (rule down_closedE)
+
+  have chF: "chain ?F"
+    apply (rule chainI)
+    apply (rule fix_on_mono2[OF pcpo_i pcpo_i cl co cl co ])
+    apply simp
+    by (rule join_mono[OF compat compat chainE[OF `chain Y`] cont2monofunE[OF `cont F`]])
+  have cho: "chain_on S' ?F"
+    apply (rule chain_onI[OF _ F_in_S'])
+    apply (rule chainE[OF chF])
+    done
+
+  have c1: "\<And> j y. chain (\<lambda>i. Y i \<squnion> F (?F j))"
+    by (rule chainI, rule join_mono[OF compat'' compat'' chainE[OF `chain Y`] below_refl])
+  have c2: "\<And> i. chain (\<lambda>j. Y i \<squnion> F (?F j))"
+    by (rule chainI, rule join_mono[OF compat'' compat'' below_refl cont2monofunE[OF `cont F` chainE[OF chF]]])
+  have c3: "chain (\<lambda>i. F (?F i))"
+    by (rule ch2ch_cont[OF `cont F` chF])
+
+  have "(\<Squnion> i. ?F i) \<in> S'"
+    by (rule chain_on_lub_on[OF cho])
+  moreover
+  {
+  have "(\<Squnion> i. Y i) \<squnion> F (\<Squnion> i. fix_on (S i) (\<lambda>x. Y i \<squnion> F x))
+    = (\<Squnion> i. Y i) \<squnion> (\<Squnion> i. F (fix_on (S i) (\<lambda>x. Y i \<squnion> F x)))"
+    by (subst cont_on2contlubE[OF coF cho], rule)
+  also have " ... = (\<Squnion> i. Y i \<squnion> (\<Squnion> i. F (fix_on (S i) (\<lambda>x. Y i \<squnion> F x))))"
+    by (rule join_cont1[OF `chain Y` admD[OF compatible_adm2 c3 compat'']])
+  also have " ... = (\<Squnion> i j. Y i \<squnion> F (fix_on (S j) (\<lambda>x. Y j \<squnion> F x)))"
+    by (subst join_cont2[OF c3 compat''], rule)
+  also have " ... = (\<Squnion> i. Y i \<squnion> F (fix_on (S i) (\<lambda>x. Y i \<squnion> F x)))"
+    by (rule diag_lub[OF c1 c2])
+  also have " ... = (\<Squnion> i. fix_on (S i) (\<lambda>x. Y i \<squnion> F x))"
+    by (subst subpcpo.fix_on_eq[symmetric, OF pcpo_i co cl], rule)
+  also note calculation
+  }
+  hence "(\<Squnion> i. Y i) \<squnion> F (\<Squnion> i. fix_on (S i) (\<lambda>x. Y i \<squnion> F x)) \<sqsubseteq> (\<Squnion> i. fix_on (S i) (\<lambda>x. Y i \<squnion> F x))"
+    by simp
+  ultimately
+  show ?thesis
+   by (rule fix_on_least_below[OF co' cl'])
+qed
+
+lemma "compatible_fmap a b \<Longrightarrow> compatible a b"
+  unfolding compatible_def
+  apply (rule exI[where x = "fmap_join a b"] )
+  apply (rule is_lubI)
+  apply (rule is_ubI)
+  apply auto
+  oops
+
+lemma heapExtendJoin_cont':
+  assumes "\<And> e. e \<in> snd ` set h \<Longrightarrow> cont (ESem e)"
+  shows "cont (\<lambda>\<rho>. heapExtendJoin \<rho> h ESem)"
+proof (rule contI2)
+case goal1 show ?case using assms by (metis heapExtendJoin_mono') 
+next
+case (goal2 Y)
+  hence [simp]:"\<And> i. fdom (Y i) = fdom (\<Squnion> i. Y i)" (is "\<And> _ .(_ = ?d)") by (metis chain_fdom)
+
+  show ?case
+  proof(cases "?d \<inter> (fst ` set h) = {}")
+  case True[simp]
+    (* Approach by finding compatible pcpo's: *)
+
+    have "fix_on (compatible_with_heap_and_env h ESem (Lub Y)) (\<lambda>\<rho>'. fmap_join (Lub Y) (heapToEnv h (\<lambda>e. ESem e \<rho>'))) \<sqsubseteq>
+      (\<Squnion> i. fix_on (compatible_with_heap_and_env h ESem (Lub Y)) (\<lambda>\<rho>'. fmap_join (Y i) (heapToEnv h (\<lambda>e. ESem e \<rho>'))))"
+      apply (rule fix_on_cont''[OF `chain Y` subpcpo_compat_h_e])
+      sorry
+
+    show ?thesis
+      unfolding heapExtendJoin_def3
+      unfolding heapExtendJoin_cond_def
+      apply (simp)
+      apply (rule fix_on_cont'[OF `chain Y` subpcpo_compat_h_e closed_on_compat_h_e cont_on_compat_h_e])
+      defer
+      apply (simp add: bottom_of_compat_h_e)
+      sorry
+  next
+  case False
+    thus ?thesis
+      unfolding heapExtendJoin_def3
+      unfolding heapExtendJoin_cond_def
+      by simp
+  qed
+qed
+
+
+lemma heapExtendJoin_cont'':
+  "\<lbrakk> (\<And> e. e \<in> snd ` set h \<Longrightarrow> cont (ESem e));
+    fdom (Y 0) \<inter> (fst ` set h) = {} \<rbrakk>
+  \<Longrightarrow> range (\<lambda>i. heapExtendJoin (Y i) h ESem) <<| heapExtendJoin (\<Squnion> i. Y i) h ESem"
 sorry
 
 
